Add the extracted handoff acceptance checker to scheduling theory
Extend the Awkernel handoff trace family with a computable acceptance path, wire the captured handoff witness to the generated post-state path, and register the extraction driver in _CoqProject. This makes the acceptance-checking milestone self-contained on the theory side rather than relying on uncommitted local files.

Add the Haskell extraction entrypoint, generated checker module, and a local make target for refreshing the extracted artifact. The committed extraction artifact now matches the awkernel acceptance tooling, while draft plan/task files remain intentionally untracked.

extracted/haskell/AwkernelHandoffAcceptance.hs
@@ -1,0 +1,382 @@
+module AwkernelHandoffAcceptance where
+
+import qualified Prelude
+
+data Bool =
+   True
+ | False
+
+andb :: Bool -> Bool -> Bool
+andb b1 b2 =
+  case b1 of {
+   True -> b2;
+   False -> False}
+
+data Nat =
+   O
+ | S Nat
+
+data Option a =
+   Some a
+ | None
+
+data List a =
+   Nil
+ | Cons a (List a)
+
+eqb :: Bool -> Bool -> Bool
+eqb b1 b2 =
+  case b1 of {
+   True -> b2;
+   False -> case b2 of {
+             True -> False;
+             False -> True}}
+
+eqb0 :: Nat -> Nat -> Bool
+eqb0 n m =
+  case n of {
+   O -> case m of {
+         O -> True;
+         S _ -> False};
+   S n' -> case m of {
+            O -> False;
+            S m' -> eqb0 n' m'}}
+
+type JobId = Nat
+
+type CPU = Nat
+
+data OpEvent =
+   EvWakeup JobId
+ | EvBlock JobId
+ | EvComplete JobId
+ | EvRequestResched CPU
+ | EvHandleResched CPU
+ | EvChoose CPU JobId
+ | EvDispatch CPU JobId
+ | EvPreempt CPU JobId JobId
+ | EvStutter
+ | EvTick
+
+data AwkernelState =
+   MkAwkernelState (CPU -> Option JobId) (List JobId) (CPU -> Bool) (CPU ->
+                                                                    Option
+                                                                    JobId)
+
+data AwkernelCapturedRow =
+   MkAwkernelCapturedRow CPU OpEvent (Option JobId) (List JobId) Bool 
+ (Option JobId)
+
+acr_cpu :: AwkernelCapturedRow -> CPU
+acr_cpu a =
+  case a of {
+   MkAwkernelCapturedRow acr_cpu0 _ _ _ _ _ -> acr_cpu0}
+
+acr_event :: AwkernelCapturedRow -> OpEvent
+acr_event a =
+  case a of {
+   MkAwkernelCapturedRow _ acr_event0 _ _ _ _ -> acr_event0}
+
+acr_current :: AwkernelCapturedRow -> Option JobId
+acr_current a =
+  case a of {
+   MkAwkernelCapturedRow _ _ acr_current0 _ _ _ -> acr_current0}
+
+acr_runnable :: AwkernelCapturedRow -> List JobId
+acr_runnable a =
+  case a of {
+   MkAwkernelCapturedRow _ _ _ acr_runnable0 _ _ -> acr_runnable0}
+
+acr_need_resched :: AwkernelCapturedRow -> Bool
+acr_need_resched a =
+  case a of {
+   MkAwkernelCapturedRow _ _ _ _ acr_need_resched0 _ -> acr_need_resched0}
+
+acr_dispatch_target :: AwkernelCapturedRow -> Option JobId
+acr_dispatch_target a =
+  case a of {
+   MkAwkernelCapturedRow _ _ _ _ _ acr_dispatch_target0 ->
+    acr_dispatch_target0}
+
+awk_baseline_state0 :: AwkernelState
+awk_baseline_state0 =
+  MkAwkernelState (\_ -> None) Nil (\_ -> False) (\_ -> None)
+
+awk_baseline_state1 :: AwkernelState
+awk_baseline_state1 =
+  MkAwkernelState (\_ -> None) (Cons (S O) Nil) (\_ -> False) (\_ -> None)
+
+awk_baseline_state3 :: AwkernelState
+awk_baseline_state3 =
+  MkAwkernelState (\c ->
+    case eqb0 c (S O) of {
+     True -> Some (S O);
+     False -> None}) Nil (\_ -> False) (\_ -> None)
+
+awk_baseline_state4 :: AwkernelState
+awk_baseline_state4 =
+  MkAwkernelState (\_ -> None) Nil (\c -> eqb0 c (S O)) (\_ -> None)
+
+data AwkernelHandoffState =
+   MkAwkernelHandoffState AwkernelState Nat
+
+awk_handoff_phase :: AwkernelHandoffState -> Nat
+awk_handoff_phase a =
+  case a of {
+   MkAwkernelHandoffState _ awk_handoff_phase0 -> awk_handoff_phase0}
+
+awk_handoff_state0 :: AwkernelHandoffState
+awk_handoff_state0 =
+  MkAwkernelHandoffState awk_baseline_state0 O
+
+awk_handoff_state1 :: AwkernelHandoffState
+awk_handoff_state1 =
+  MkAwkernelHandoffState awk_baseline_state1 (S O)
+
+awk_handoff_request_visible :: AwkernelState
+awk_handoff_request_visible =
+  MkAwkernelState (\_ -> None) (Cons (S O) Nil) (\c -> eqb0 c (S O)) (\_ ->
+    None)
+
+awk_handoff_state2 :: AwkernelHandoffState
+awk_handoff_state2 =
+  MkAwkernelHandoffState awk_handoff_request_visible (S (S O))
+
+awk_handoff_state3 :: AwkernelHandoffState
+awk_handoff_state3 =
+  MkAwkernelHandoffState awk_handoff_request_visible (S (S (S O)))
+
+awk_handoff_choose_visible :: AwkernelState
+awk_handoff_choose_visible =
+  MkAwkernelState (\_ -> None) (Cons (S O) Nil) (\c -> eqb0 c (S O)) (\c ->
+    case eqb0 c (S O) of {
+     True -> Some (S O);
+     False -> None})
+
+awk_handoff_state4 :: AwkernelHandoffState
+awk_handoff_state4 =
+  MkAwkernelHandoffState awk_handoff_choose_visible (S (S (S (S O))))
+
+awk_handoff_state5 :: AwkernelHandoffState
+awk_handoff_state5 =
+  MkAwkernelHandoffState awk_baseline_state3 (S (S (S (S (S O)))))
+
+awk_handoff_state6 :: AwkernelHandoffState
+awk_handoff_state6 =
+  MkAwkernelHandoffState awk_baseline_state4 (S (S (S (S (S (S O))))))
+
+op_event_eqb :: OpEvent -> OpEvent -> Bool
+op_event_eqb x y =
+  case x of {
+   EvWakeup j1 -> case y of {
+                   EvWakeup j2 -> eqb0 j1 j2;
+                   _ -> False};
+   EvBlock j1 -> case y of {
+                  EvBlock j2 -> eqb0 j1 j2;
+                  _ -> False};
+   EvComplete j1 -> case y of {
+                     EvComplete j2 -> eqb0 j1 j2;
+                     _ -> False};
+   EvRequestResched c1 ->
+    case y of {
+     EvRequestResched c2 -> eqb0 c1 c2;
+     _ -> False};
+   EvHandleResched c1 ->
+    case y of {
+     EvHandleResched c2 -> eqb0 c1 c2;
+     _ -> False};
+   EvChoose c1 j1 ->
+    case y of {
+     EvChoose c2 j2 -> andb (eqb0 c1 c2) (eqb0 j1 j2);
+     _ -> False};
+   EvDispatch c1 j1 ->
+    case y of {
+     EvDispatch c2 j2 -> andb (eqb0 c1 c2) (eqb0 j1 j2);
+     _ -> False};
+   EvPreempt c1 old1 new1 ->
+    case y of {
+     EvPreempt c2 old2 new2 ->
+      andb (andb (eqb0 c1 c2) (eqb0 old1 old2)) (eqb0 new1 new2);
+     _ -> False};
+   EvStutter -> case y of {
+                 EvStutter -> True;
+                 _ -> False};
+   EvTick -> case y of {
+              EvTick -> True;
+              _ -> False}}
+
+awk_handoff_row_wakeup :: AwkernelCapturedRow
+awk_handoff_row_wakeup =
+  MkAwkernelCapturedRow O (EvWakeup (S O)) None (Cons (S O) Nil) False None
+
+awk_handoff_row_request_resched :: AwkernelCapturedRow
+awk_handoff_row_request_resched =
+  MkAwkernelCapturedRow (S O) (EvRequestResched (S O)) None (Cons (S O) Nil)
+    True None
+
+awk_handoff_row_handle_resched :: AwkernelCapturedRow
+awk_handoff_row_handle_resched =
+  MkAwkernelCapturedRow (S O) (EvHandleResched (S O)) None (Cons (S O) Nil)
+    True None
+
+awk_handoff_row_choose :: AwkernelCapturedRow
+awk_handoff_row_choose =
+  MkAwkernelCapturedRow (S O) (EvChoose (S O) (S O)) None (Cons (S O) Nil)
+    True (Some (S O))
+
+awk_handoff_row_dispatch :: AwkernelCapturedRow
+awk_handoff_row_dispatch =
+  MkAwkernelCapturedRow (S O) (EvDispatch (S O) (S O)) (Some (S O)) Nil False
+    None
+
+awk_handoff_row_complete :: AwkernelCapturedRow
+awk_handoff_row_complete =
+  MkAwkernelCapturedRow (S O) (EvComplete (S O)) None Nil True None
+
+option_job_eqb :: (Option JobId) -> (Option JobId) -> Bool
+option_job_eqb x y =
+  case x of {
+   Some j1 -> case y of {
+               Some j2 -> eqb0 j1 j2;
+               None -> False};
+   None -> case y of {
+            Some _ -> False;
+            None -> True}}
+
+job_list_eqb :: (List JobId) -> (List JobId) -> Bool
+job_list_eqb xs ys =
+  case xs of {
+   Nil -> case ys of {
+           Nil -> True;
+           Cons _ _ -> False};
+   Cons x xs' ->
+    case ys of {
+     Nil -> False;
+     Cons y ys' -> andb (eqb0 x y) (job_list_eqb xs' ys')}}
+
+captured_row_eqb :: AwkernelCapturedRow -> AwkernelCapturedRow -> Bool
+captured_row_eqb x y =
+  andb
+    (andb
+      (andb
+        (andb
+          (andb (eqb0 (acr_cpu x) (acr_cpu y))
+            (op_event_eqb (acr_event x) (acr_event y)))
+          (option_job_eqb (acr_current x) (acr_current y)))
+        (job_list_eqb (acr_runnable x) (acr_runnable y)))
+      (eqb (acr_need_resched x) (acr_need_resched y)))
+    (option_job_eqb (acr_dispatch_target x) (acr_dispatch_target y))
+
+awk_handoff_row_step_next :: AwkernelHandoffState -> AwkernelCapturedRow ->
+                             Option AwkernelHandoffState
+awk_handoff_row_step_next st row =
+  case captured_row_eqb row awk_handoff_row_wakeup of {
+   True ->
+    case awk_handoff_phase st of {
+     O -> Some awk_handoff_state1;
+     S _ -> None};
+   False ->
+    case captured_row_eqb row awk_handoff_row_request_resched of {
+     True ->
+      case awk_handoff_phase st of {
+       O -> None;
+       S n -> case n of {
+               O -> Some awk_handoff_state2;
+               S _ -> None}};
+     False ->
+      case captured_row_eqb row awk_handoff_row_handle_resched of {
+       True ->
+        case awk_handoff_phase st of {
+         O -> None;
+         S n ->
+          case n of {
+           O -> None;
+           S n0 -> case n0 of {
+                    O -> Some awk_handoff_state3;
+                    S _ -> None}}};
+       False ->
+        case captured_row_eqb row awk_handoff_row_choose of {
+         True ->
+          case awk_handoff_phase st of {
+           O -> None;
+           S n ->
+            case n of {
+             O -> None;
+             S n0 ->
+              case n0 of {
+               O -> None;
+               S n1 ->
+                case n1 of {
+                 O -> Some awk_handoff_state4;
+                 S _ -> None}}}};
+         False ->
+          case captured_row_eqb row awk_handoff_row_dispatch of {
+           True ->
+            case awk_handoff_phase st of {
+             O -> None;
+             S n ->
+              case n of {
+               O -> None;
+               S n0 ->
+                case n0 of {
+                 O -> None;
+                 S n1 ->
+                  case n1 of {
+                   O -> None;
+                   S n2 ->
+                    case n2 of {
+                     O -> Some awk_handoff_state5;
+                     S _ -> None}}}}};
+           False ->
+            case captured_row_eqb row awk_handoff_row_complete of {
+             True ->
+              case awk_handoff_phase st of {
+               O -> None;
+               S n ->
+                case n of {
+                 O -> None;
+                 S n0 ->
+                  case n0 of {
+                   O -> None;
+                   S n1 ->
+                    case n1 of {
+                     O -> None;
+                     S n2 ->
+                      case n2 of {
+                       O -> None;
+                       S n3 ->
+                        case n3 of {
+                         O -> Some awk_handoff_state6;
+                         S _ -> None}}}}}};
+             False -> None}}}}}}
+
+awk_handoff_generate_post_states_from :: AwkernelHandoffState -> (List
+                                         AwkernelCapturedRow) -> Option
+                                         (List AwkernelHandoffState)
+awk_handoff_generate_post_states_from st rows =
+  case rows of {
+   Nil -> Some Nil;
+   Cons row rows' ->
+    case awk_handoff_row_step_next st row of {
+     Some st' ->
+      case awk_handoff_generate_post_states_from st' rows' of {
+       Some states -> Some (Cons st' states);
+       None -> None};
+     None -> None}}
+
+awk_handoff_generate_post_states :: (List AwkernelCapturedRow) -> Option
+                                    (List AwkernelHandoffState)
+awk_handoff_generate_post_states rows =
+  awk_handoff_generate_post_states_from awk_handoff_state0 rows
+
+awk_handoff_check_rows :: (List AwkernelCapturedRow) -> Option
+                          (List AwkernelHandoffState)
+awk_handoff_check_rows =
+  awk_handoff_generate_post_states
+
+awk_handoff_accepts_rows :: (List AwkernelCapturedRow) -> Bool
+awk_handoff_accepts_rows rows =
+  case awk_handoff_check_rows rows of {
+   Some _ -> True;
+   None -> False}
+
